examples/ProcTwoStInl.v
@@ -20,11 +20,13 @@ Section Inlined.
             (getSrc1: Src1T lgDataBytes rfIdx)
             (getSrc2: Src2T lgDataBytes rfIdx)
             (execState: ExecStateT addrSize lgDataBytes rfIdx)
-            (execNextPc: ExecNextPcT addrSize lgDataBytes rfIdx).
+            (execNextPc: ExecNextPcT addrSize lgDataBytes rfIdx)
+            (predictNextPc: forall ty, fullType ty (SyntaxKind (Bit addrSize)) -> (* pc *)
+                                       Expr ty (SyntaxKind (Bit addrSize))).
 
   Definition p2st := p2st getOptype getLdDst getLdAddr getLdSrc calcLdAddr
                           getStAddr getStSrc calcStAddr getStVSrc
-                          getSrc1 execState execNextPc.
+                          getSrc1 execState execNextPc predictNextPc.
   Hint Unfold p2st: ModuleDefs. (* for kinline_compute *)
 
   Definition p2stInl: sigT (fun m: Modules => p2st <<== m).
@@ -32,7 +34,8 @@ Section Inlined.
     pose proof (inlineF_refines
                   (procTwoStage_ModEquiv getOptype getLdDst getLdAddr getLdSrc calcLdAddr
                                          getStAddr getStSrc calcStAddr getStVSrc
-                                         getSrc1 execState execNextPc type typeUT)
+                                         getSrc1 execState execNextPc predictNextPc
+                                         type typeUT)
                   (Reflection.noDupStr_NoDup (Struct.namesOf (getDefsBodies p2st)) eq_refl))
       as Him.
     unfold MethsT in Him; rewrite <-SemFacts.idElementwiseId in Him.
@@ -44,16 +47,6 @@ Section Inlined.
     specialize (Him eq_refl).
     exact (existT _ _ Him).
   Defined.
-
-  (* Definition p2stInl: Modules * bool. *)
-  (* Proof. *)
-  (*   remember (inlineF p2st) as inlined. *)
-  (*   kinline_compute_in Heqinlined. *)
-  (*   match goal with *)
-  (*   | [H: inlined = ?m |- _] => *)
-  (*     exact m *)
-  (*   end. *)
-  (* Defined. *)
 
 End Inlined.
 
